theories/examples/cell.v
@@ -7,9 +7,7 @@ From reloc.lib Require Export lock.
 (** A type of cells -- basically an abstract type of references. *)
 (* ∀ α, ∃ β, (α → β) × (β → α) × (β → α → ())  *)
 Definition cellτ : type :=
-  ∀: ∃: (TVar 1 → TVar 0)
-       * (TVar 0 → TVar 1)
-       * (TVar 0 → TVar 1 → TUnit).
+  ∀: ∃: (#1 → #0) * (#0 → #1) * (#0 → #1 → ()).
 (** We show that the canonical implementation `cell1` is equivalent to
 an implementation using two alternating slots *)
 
